\documentclass[12pt]{article}

\usepackage[margin=1in]{geometry}
\usepackage[protrusion=true,expansion=true]{microtype}
\usepackage{lmodern}
\usepackage{amsmath}
\DeclareMathOperator{\sech}{sech}
\DeclareMathOperator{\invcos}{cos^{-1}}

\linespread{1.6}
\setlength\parindent{0em}

\newcommand{\bfit}[2]{\textbf{#1}\ \textit{#2}}
\renewcommand{\title}[2]{\huge\bfit{#1}{#2}\normalsize}
\newcommand{\double}[0]{\par\null\par}
\renewcommand{\section}[2]{\double\LARGE\bfit{#1}{\##2}\normalsize\\}
\renewcommand{\exp}[1]{e^{#1}}
\newcommand{\paren}[1]{\left({#1}\right)}
\let\infinity\infty
\let\xint\int
\renewcommand{\int}[2]{\xint{#1}\,d#2}

\begin{document}
\fontfamily{lmr}\selectfont
\title{10 detailed solutions}{by Spencer Todd}
\section{6.1}{39}
Find $\paren{f^{-1}}'\paren{a}$ if $f\paren{x}=3x^3+4x^2+6x+5$ and $a=5$.\double

Theorem 7 in Section 6.1 establishes that if $f$ is one-to-one, its inverse is
$f^{-1}$, and \\$f'\paren{f^{-1}\paren{a}}\neq 0$, then
%
\begin{equation*}
\paren{f^{-1}}'\paren{a}=\frac{1}{f'\paren{f^{-1}\paren{a}}}.
\end{equation*}

(A glance at $f'$ indicates that $f$ is monotonic increasing.) First, we must find the derivative of $f\paren{x}$, then apply Theorem 7. Additionally, $f\paren{x}=5$ when $x=0$, so
$f^{-1}\paren{5}=0$.
%
\begin{align*}
f'\paren{x}&=9x^2+8x+6 \\
%
\paren{f^{-1}}'\paren{a}&=\frac{1}{f'\paren{f^{-1}\paren{5}}} \\
&=\frac{1}{f'\paren{0}} \\
&=\frac{1}{6}
\end{align*}

\section{6.8}{29}
Find the limit:
%
\begin{equation*}
\lim_{x\to 0}\frac{\tanh{x}}{\tan{x}}.
\end{equation*}\double

Since $\displaystyle\lim_{x\to 0}\tanh{x}=0$ and $\displaystyle\lim_{x\to 0}\tan{x}=0$, this limit is of the
$\frac{0}{0}$ indeterminate form, so we can use L'H\^{o}pital's Rule.
%
\begin{align*}
&\lim_{x\to 0}\frac{\frac{d}{dx}\tanh{x}}{\frac{d}{dx}\tan{x}} \\
&\lim_{x\to 0}\frac{\sech^2 x}{\sec^2 x} \\
&\frac{1^2}{1^2} \\
&1
\end{align*}

\section{7.1}{9}
Evaluate the integral:
%
\begin{equation*}
\int{\invcos{x}}{x}.
\end{equation*}\double

Since $\invcos{x}$ has an easy derivative, we can use integration by parts by differentiating $\invcos{x}$ and integrating $dx$.
%
\begin{equation*}
\int{u}{v}=u\,v-\int{v}{u}
\end{equation*}
%
\begin{alignat*}{2}
u&=\invcos{x} &\quad dv&=dx \\
du&=\frac{-dx}{\sqrt{1-x^2}} &\quad v&=x
\end{alignat*}
%
\begin{align*}
\int{\invcos{x}}{x}&=x\invcos{x}-\int{\frac{-x}{\sqrt{1-x^2}}}{x}
\end{align*}
%
We can set everything inside the radical to a new variable, $a$.
%
\begin{align*}
a&=1-x^2 \\
da&=-2x\,dx \\
\frac{da}{2}&=-x\,dx
\end{align*}
%
\begin{align*}
\int{\invcos{x}}{x}&=x\invcos{x}-\xint{\frac{da}{2\sqrt{a}}} \\
&=x\invcos{x}-\sqrt{a}+C \\
&=x\invcos{x}-\sqrt{1-x^2}+C
\end{align*}

\section{7.2}{1}
Evaluate the integral:
%
\begin{equation*}
\int{\sin^2{x}\cos^3{x}}{x}.
\end{equation*}\double

Since the power of $\cos$ is odd, the substitution $z=\sin{x}$ will work.
%
\begin{align*}
z&=\sin{x} \\
\frac{dz}{dx}&=\cos{x} \\
dx&=\frac{dz}{\cos{x}}
\end{align*}

We can use a trigonometric identity to handle the $\cos$.
%
\begin{align*}
\sin^2{x}+\cos^2{x}&=1 \\
\cos^2{x}&=1-\sin^2{x} \\
&=1-z^2
\end{align*}

Arranging the expression as follows will highlight our choices of substitutions:
%
\begin{align*}
\int{\sin^2{x}\cos^3{x}}{x}&=\xint\paren{\sin{x}}^2\paren{\cos^2{x}}\paren{\cos{x}\,dx}. \\
&=\xint{z}^2\paren{1-z^2}\paren{\cos{x}\,\frac{dz}{\cos{x}}} \\
&=\int{z^2-z^4}{z}
\intertext{Now we may finish the integral using the power rule and substitution.}
&=\frac{z^3}{3}-\frac{z^5}{5}+C \\
&=\frac{\sin^3{x}}{3}-\frac{\sin^5{x}}{5}+C
\end{align*}

\section{9.5}{7}
Solve the differential equation:
%
\begin{equation*}
y'+y=x. \tag{1}
\end{equation*}\double
We are given an inhomogenous equation, so we must first solve the corresponding homogenous equation:
%
\begin{align*}
\frac{dy_0}{dx}+y_0&=0. \\
\frac{dy_0}{y_0}&=-dx \\
\xint\frac{dy_0}{y_0}&=-\xint{dx} \\
\ln{|y_0|}&=-x+A \\
|y_0|&=\exp{-x+A} \\
y_0&=B\exp{-x}\text{, whereas $B=\pm\exp{A}$}
%
\intertext{Returning to the original equation, we can replace the constant $B$ with a differentiable function, $u$.}
%
y&=u\,\exp{-x} \tag{2} \\
y'&=u'\exp{-x}-u\,\exp{-x} \tag{3}
%
\intertext{Now, we can plug equations (2) and (3) in to (1) and solve for $u$. Notice that a nice cancellation occurs.}
%
u'\exp{-x}-u\,\exp{-x}+u\,\exp{-x}&=x \\
u'\exp{-x}&=x \\
u'&=x\,\exp{x} \\
\xint{du}&=\int{x\,\exp{x}}{x}
\end{align*}

We may proceed using integration by parts $\paren{\int{g}{h}=g\,h-\int{h}{g}}$.
%
\begin{alignat*}{2}
g&=x &\quad dh&=\exp{x}\,dx \\
dg&=dx &\quad h&=\exp{x}
\end{alignat*}
%
\begin{align*}
u&=x\,\exp{x}-\int{\exp{x}}{x} \\
&=x\,\exp{x}-\exp{x}+C \tag{4}
\intertext{Finally, we can plug equation (4) in to (2) for our final answer.}
y&=\exp{-x}\paren{x\,\exp{x}-\exp{x}+C} \\
&=x-1+C\exp{-x}
\end{align*}

\section{10.2}{15}
Find $\displaystyle\frac{dy}{dx}$ and $\displaystyle\frac{d^2y}{dx^2}.$
%
\begin{align*}
x&=t-\ln{t} \\
y&=t+\ln{t}
\end{align*}\double

By the chain rule, $\displaystyle\frac{dy}{dx}=\frac{dy}{dt}\frac{dt}{dx}=\frac{\frac{dy}{dt}}{\frac{dx}{dt}}$.
%
\begin{align*}
\frac{dy}{dt}&=1+\frac{1}{t} \\
\frac{dx}{dt}&=1-\frac{1}{t} \\
\frac{\frac{dy}{dt}}{\frac{dx}{dt}}&=\frac{1+\frac{1}{t}}{1-\frac{1}{t}} \\
\frac{dy}{dx}&=\frac{t+1}{t-1}
\end{align*}
%
By the chain rule, $\displaystyle
\frac{d^2y}{dx^2}
=\frac{d}{dx}\frac{dy}{dx}
=\frac{d}{dt}\frac{dt}{dx}\frac{dy}{dx}
=\frac{\frac{d}{dt}\paren{\frac{dy}{dx}}}{\frac{dx}{dt}}
$.
%
\begin{align*}
\frac{d}{dt}\paren{\frac{dy}{dx}}&=\frac{\paren{t-1}\paren{1}-\paren{t+1}\paren{1}}{\paren{t-1}^2} \\
&=\frac{-2}{\paren{t-1}^2} \\
\frac{dx}{dt}&=1-\frac{1}{t} \\
\frac{\frac{d}{dt}\paren{\frac{dy}{dx}}}{\frac{dx}{dt}}&=\frac{-2}{\paren{t-1}^2}\cdot\frac{1}{1-\frac{1}{t}} \\
\frac{d^2y}{dx^2}&=\frac{-2t}{\paren{t-1}^3}
\end{align*}

\section{10.4}{2}
Find the area of the region that is bounded by the given curve and lies in the specified sector.
%
\begin{equation*}
r\paren\theta=\cos{\theta},\ 0\leq\theta\leq\frac\pi{6}
\end{equation*}\double

The area of a sector of a circle $\paren{A=\frac{1}{2}{r}^2\theta}$ leads us to the equation for the integral of polar equations:
%
\begin{align*}
&\frac{1}{2}\xint_a^b{r\paren\theta^2}\,{d\theta}. \\
\\
&\frac{1}{2}\xint_0^{\frac\pi{6}}{\cos^2\theta}\,{d\theta}
\intertext{Since the power of $\sin$ $\paren{0}$ and $\cos$ $\paren{2}$ are both even, we may proceed using the double angle
formula for cosine.}
&\frac{1}{4}\xint_0^{\frac\pi{6}}{1+\cos{2\theta}}\,{d\theta} \\
&\frac{1}{4}\left({\theta+\frac{1}{2}\sin{2\theta}}\right|_0^\frac\pi{6} \\
&\frac{1}{4}\paren{\frac\pi{6}+\frac{1}{2}\sin{\frac\pi{3}}} \\
\intertext{Notice that the expression evaluated at $0$ is $0$.}
&\frac\pi{24}+\frac{\sqrt{3}}{16}
\end{align*}

\section{11.10}{78}
Find the sum of the series.
%
\begin{align*}
&1-\ln{2}+\frac{\paren{\ln{2}}^2}{2!}-\frac{\paren{\ln{2}}^3}{3!}+\dots \\
\\
\intertext{Writing the equation for the sum will clearly show us a necessary substitution.}
&\sum_{n=0}^\infinity\paren{-1}^n\frac{\paren{\ln{2}}^n}{n!}
\intertext{Since the factors $-1$ and $\ln{2}$ both have power $n$, the $-1$ can multiply in to the numerator to make $\paren{-\ln{2}}^n$. Then we can make the substitution $x=-\ln{2}$, resulting in:}
&\sum_{n=0}^\infinity\frac{x^n}{n!}.
\intertext{We know that this is also the power series for $\exp{x}$ for all $x$. So, the solution is $\exp{x}$ evaluated at $x=-\ln{2}$, or $\frac{1}{2}$.}
\end{align*}

\end{document}
